##### Statistics 110

###### MGFs Continued

---



### Goal of this lecture

> 적률 생성 함수를 이용해 적률을 구할 수 있다. 결합 분포를 이용해 주변 분포를 구하고, 확률 분포의 독립 여부를 판단할 수 있다.







#### Exponential MGF

$$
\begin{aligned}
&X\sim Expo(1),\ find\ MGF\ moments.\\
&\to_{(by\ LOTUS)}\ M(t)=E(e^{tX})=\int_0^{\infin}e^{tX}e^{-X}dx=\int_0^{\infin}e^{-X(1-t)}dx=\bold{\frac{1}{1-t}},\ (t<1)\\
&\begin{cases}
M'(0)=E(X)\\
M''(0)=E(X^2)\\
...
\end{cases}
\quad \to\ \frac{1}{1-t}=\sum_{n=0}^{\infin}t^n=\sum_{n=0}^{\infin}n!\cdot \frac{t^n}{n!}\quad \to\quad  \bold{E(X^n)=n!}\\
\\
\\
&Y\sim Expo(\lambda),\\
&let\ X=\lambda Y\sim Expo(1),\\
\\
&\therefore Y^n=\frac{X^n}{\lambda^n}\quad \to\ \bold{E(Y^n)=\frac{n!}{\lambda^n}}

\end{aligned}
$$







#### Normal Distribution moments

$$
\begin{aligned}
&Let\ Z\sim N(0,1),\ find\ all\ its\ moments.\\
&\begin{aligned}
\to &_{(1)}\ E(Z^n)=0\ for\ n\ odd\ by\ symmetry.\\
&_{(2)}\ M(t)=e^{\frac{t^2}{2}}=\sum_{n=0}^{\infin}\frac{(t^2/2)^n}{n!}=\sum_{n=0}^{\infin}\frac{(2n!)t^{2n}}{2^nn!(2n!)}\quad \to E(Z^{2n})=\frac{(2n)!}{2^nn!}
\end{aligned}
\end{aligned}
$$







#### Poisson Distribution moments

$$
\begin{aligned}
&Let\ X\sim\ Pois(\lambda)\\
&\to\ M(t)=E(e^{tX})=\sum_{n=0}^{\infin}e^{tk}\frac{e^{-\lambda}\lambda^k}{k!}=e^{-\lambda}e^{\lambda e^t}=\bold{e^{\lambda(e^t-1)}}\\
\\
&*\ Let\ Y\sim Pois(\mu)\ indep.\ of\ X.\ Find\ distribution\ of\ X+Y.\\
&\to\ Multiply\ MGFs:\ e^{\lambda(e^t-1)}e^{\mu(e^t-1)}=e^{(\lambda+\mu)(e^t-1)}\quad \therefore \bold{X+Y\sim Pois(\lambda+\mu)}\\
\\
&\begin{aligned}
\bold{CounterExample|}\; &If\ X,Y\ dependent,\ _{(i.e.\ X=Y)}\\
&X+Y=2X\ is\ not\ poisson,\ since\ \bold{even};\ 음이\ 아닌\ 모든\ 정수\ X.\\
&(furthermore,\ E(2X)=2\lambda\; \&\; Var(2X)=4\lambda )
\end{aligned}
\end{aligned}
$$







#### Joint Distribution

$$
\begin{aligned}

&X,Y_{(r.v.s)}
\begin{cases}
joint\ CDF:\ F(x,y)=P(X\le x, Y\le y)\\
\\
joint\ PMF_{(discrete\ case)}:\ P(X=x, Y=y)\\
\\
marginal\ CDF:\ P(X\le x)\ is\ marginal\ dist.\ of\ X\\
\\
joint\ PDF_{(cont.\ case)}:\ f(x,y)\ such\ that\ P((x,y)\in B)=\int\int_Bf(x,y)dxdy\\
\\
\begin{aligned}independence:&X,Y\ indep.\ if\ and\ only\ if\ F(x,y)=F_X(x)F_Y(y),\\ &equive.\ to\ P(X=x, Y=y)_{(discrete\ case)}=P(X=x)P(Y=y)\\ &\qquad \qquad \ \ f(x,y)=f_X(x)f_Y(y)\ for\ all\ x,y \end{aligned}

\end{cases}\\
\\
&\begin{aligned}Getting\ marginals \to\ &P(X=x)=\sum_yP(X=x, Y=y)\quad _{(disrete\ case)}\\
&f_Y(y)=\int_{-\infin}^{\infin}f_{X,Y}(x,y)dx\quad _{(cont. case)}
\end{aligned}
\\
\\
\\
&
\begin{aligned}
\bold{EX|}&\bold{(indep. case)}\ Uniform\ on\ square\{(x,y):x,y\in [0,1]\}\\
\\
&joint\ PDF 
\begin{cases}
c,\ (0\le x\le 1,\ 0\le y\le 1;\ on\ the\ square)\\
0,\ otherwise(;\ outside)
\end{cases}
\\
&\to integral\ area,\ c=\frac{1}{area}=1\\
\\
&\bold{(dependent\ case)}\ Unif\ in\ disc\ x^2+y^2\le1\\
\\
&joint\ PDF
\begin{cases}
\frac{1}{\pi},\ (x^2+y^2\le1)\\
0,\ otherwise
\end{cases}\\
&\to X,Y\ are\ dependent\ (\because Given\ X=x,\ -\sqrt{1-x^2} \le y\le \sqrt{1-x^2})

\end{aligned}

\end{aligned}
$$