##### Statistics 110

###### Conditional Expectation given an R.V.

---



### Goal of this lecture

> 조건부 기댓값의 여러 가지 성질을 이해하고 활용할 수 있다.









#### Example of Conditional Expectation

$$
\begin{aligned}
&\bold{EX_1}\quad Let\ X\sim N(0,1)\ and\ Y=X^2.\ Find\ E(Y|X),\ E(X|Y)\\
\\
&\begin{aligned}
\bold{Sol)}\quad &1.\ E(Y|X)=E(X^2|X)=X^2=Y\\
&2.\ E(X|Y)=E(X|X^2)=0\quad since\ if\ observe\ X^2=a,\ then,\ X=\pm\sqrt{a},\ equally\ likely\\
\end{aligned}\\
\\
\\
&\begin{aligned}
\bold{EX_2}\quad &A\ stick\ length\ [0,1],\ break\ off\ piece,\ and\ break\ off\ another\ piece.\\&(X\sim Unif(0,1),\ Y|X\sim Unif(0,X))\ Then,\ find\ E(Y|X=x).
\end{aligned}\\
\\
&\begin{aligned}
\bold{Sol)}\quad &E(Y|X=x)=\frac{x}{2},\ so\ E(Y|X)=\frac{X}{2}.\\
&E(\ E(Y|X)\ )=\frac{1}{2}\cdot \frac{1}{2}=\frac{1}{4}=E(Y) \\
\end{aligned}\\


\end{aligned}
$$







#### Useful Properties of Conditional Expectation

$$
\begin{aligned}
&(1)\ E(\ h(X)Y|X\ )=h(X)E(Y|X)\quad [taking\ out\ what's\ known]\ _{(e.g.\ E(X^2|X)=X^2E(1|X))}\\
&(2)\ E(Y|X)=E(Y)\quad if\ X,Y\ are\ independent\\
&(3)\ E(\ E(Y|X)\ )=E(Y)\quad [Iterated\ E\ /\ Adam's\ Law]\ _{^*E(Y)=E(E(Y|X));\ LOTP}\\
&\qquad \begin{aligned}Proof)\ &Let\ E(Y|X)=g(X)\ _{[discrete\ case]}\\
&\begin{aligned}E(g(X))=\displaystyle\sum_{x}g(x)P(X=x)&=\displaystyle\sum_{x}E(Y|X=x)P(X=x)\quad _{(\to\ by\ LOTUS\ \&\ Def)}\\&=\displaystyle\sum_{x}(\displaystyle\sum_{y}yP(Y=y|X=x)P(X=x))\\&=\displaystyle\sum_{y}\displaystyle\sum_{x}yP(Y=y,\ X=x)\\&=\displaystyle\sum_{y}y\displaystyle\sum_{x}P(Y=y,X=x)\\&=\displaystyle\sum_{y}yP(Y=y)=E(Y)\end{aligned}\end{aligned}\\
&(4)\ E(\ (Y-E(Y|X)\ )\ h(X))=0\quad _{i.e.\ Y-E(Y|X)\ is\ uncorrelated\ with\ h(X).\ (Y-E(Y|X)\to\ residual(잔차)\ )}\\
&\qquad \because Cov(Y-E(Y|X),\ h(X))=E(\ (Y-E(Y|X))\ h(X)\ )-\cancel{E(Y-E(Y|X))}_{_{\to\ 0}}E(h(X))\\
&\qquad \begin{aligned}Proof)\ E(Y\cdot h(X))-E(\ E(Y|X)h(X)\ )&=E(Y\cdot h(X))-E(\ E(h(X))Y|X\ )\\&=E(Y\cdot h(X))-E(Y\cdot h(X))=0\ \because\ by\ (3)  \end{aligned}\\
&(5)\ Var(Y)=E(Var(Y|X))_{_{그룹\ 안}}+Var(E(Y|X))_{_{그룹\ 간}}\quad [Eve's\ Law]\\
&\qquad ^{*\bold{Def}\quad Var(Y|X)=E(Y^2|X)-(E(Y|X))^2=E(\ (Y-E(Y|X))^2\ |X\ )}\\
\end{aligned}
$$






$$
\begin{aligned}

&\begin{aligned}
\bold{EX}\quad &Pick\ random\ city,\ and\ pick\ random\ sample\ of\ n\ people\ in\ that\ city\\
&X=(\#\ with\ disease),\ Q=(proportion\ of\ people\ in\ the\ random\ city\ with\ disease)\\
&Find\ E(X),\ Var(X),\ assuming\ Q\sim Beta(a,b),\ X|Q\sim Bin(n,Q)
\end{aligned}\\
\\
&\bold{Sol)}\\
&\qquad E(X)=E(\ E(X|Q)\ )=E(nQ)=\frac{na}{a+b}\\
&\qquad Var(X)=E(Var(X|Q))+Var(E(X|Q))=\underline{E(nQ(1-Q))}^{^{(1)}}+\underline{n^2Var(Q)}^{^{(2)}}\\
\\
&\qquad \begin{aligned}^{^{(1)}}E(nQ(1-Q))&=\frac{\Gamma(a+b)}{\Gamma(a)\Gamma(b)}\int_{0}^{1}q(1-q)q^{a-1}(1-q)^{b-1}dq\\&=\frac{\Gamma(a+b)}{\Gamma(a)\Gamma(b)}\cdot \frac{\Gamma(a+1)\Gamma{(b+1)}}{\Gamma(a+b+2)}=\frac{ab\cancel{\Gamma(a+b)}}{(a+b+1)(a+b)\cancel{\Gamma(a+b)}} \end{aligned}\\
&\qquad \begin{aligned}^{^{(2)}}Var(Q)=\frac{\mu(1-\mu)}{a+b+1},\quad where\ \mu=\frac{a}{a+b}\end{aligned}


\end{aligned}
$$

